finished proof of lemma 5.5.9

ASC_Suite.thy
@@ -269,32 +269,33 @@ abbreviation append_sets :: "'a list set \<Rightarrow> 'a list set \<Rightarrow>
    C  = currently considered sequences
    RM = sequences to remove
 *)
-fun TS :: "('in, 'out, 'state1) FSM \<Rightarrow> ('in, 'out, 'state2) FSM \<Rightarrow> 'in list set \<Rightarrow> 'state1 set \<Rightarrow> ('in, 'out) ATC set \<Rightarrow> 'in list set \<Rightarrow> nat \<Rightarrow> nat \<Rightarrow> 'in list set" 
-and C  :: "('in, 'out, 'state1) FSM \<Rightarrow> ('in, 'out, 'state2) FSM \<Rightarrow> 'in list set \<Rightarrow> 'state1 set \<Rightarrow> ('in, 'out) ATC set \<Rightarrow> 'in list set \<Rightarrow> nat \<Rightarrow> nat \<Rightarrow> 'in list set"   
-and RM :: "('in, 'out, 'state1) FSM \<Rightarrow> ('in, 'out, 'state2) FSM \<Rightarrow> 'in list set \<Rightarrow> 'state1 set \<Rightarrow> ('in, 'out) ATC set \<Rightarrow> 'in list set \<Rightarrow> nat \<Rightarrow> nat \<Rightarrow> 'in list set"   
+fun TS :: "('in, 'out, 'state1) FSM \<Rightarrow> ('in, 'out, 'state2) FSM \<Rightarrow> 'in list set \<Rightarrow> ('in, 'out) ATC set \<Rightarrow> 'in list set \<Rightarrow> nat \<Rightarrow> nat \<Rightarrow> 'in list set" 
+and C  :: "('in, 'out, 'state1) FSM \<Rightarrow> ('in, 'out, 'state2) FSM \<Rightarrow> 'in list set \<Rightarrow> ('in, 'out) ATC set \<Rightarrow> 'in list set \<Rightarrow> nat \<Rightarrow> nat \<Rightarrow> 'in list set"   
+and RM :: "('in, 'out, 'state1) FSM \<Rightarrow> ('in, 'out, 'state2) FSM \<Rightarrow> 'in list set \<Rightarrow> ('in, 'out) ATC set \<Rightarrow> 'in list set \<Rightarrow> nat \<Rightarrow> nat \<Rightarrow> 'in list set"   
 where
-  "RM M2 M1 T S \<Omega> V m 0 = {}" |
-  "TS M2 M1 T S \<Omega> V m 0 = {}" |
-  "TS M2 M1 T S \<Omega> V m (Suc 0) = V" |
-  "C M2 M1 T S \<Omega> V m 0 = {}" |
-  "C M2 M1 T S \<Omega> V m (Suc 0) = V" |
-  "RM M2 M1 T S \<Omega> V m (Suc n) = 
-    {xs' \<in> C M2 M1 T S \<Omega> V m (Suc n) .
-      (\<forall> io \<in> language_state_in M1 (initial M1) {xs'} .
-        (\<exists> V'' \<in> N io M1 V .  
-          (\<exists> S1 . 
-            (\<exists> vs xs .
-              io = (vs@xs)
-              \<and> mcp (vs@xs) V'' vs
-              \<and> S1 \<subseteq> S
-              \<and> (\<forall> s1 \<in> S1 . \<forall> s2 \<in> S1 .
-                s1 \<noteq> s2 \<longrightarrow> 
-                  (\<forall> io1 \<in> RP M2 s1 vs xs V'' .
-                     \<forall> io2 \<in> RP M2 s2 vs xs V'' .
-                       B M1 io1 \<Omega> \<noteq> B M1 io2 \<Omega> ))
-              \<and> m < LB M2 M1 vs xs T S \<Omega> V'' ))))}" |
-  "C M2 M1 T S \<Omega> V m (Suc n) = (append_set ((C M2 M1 T S \<Omega> V m n) - (RM M2 M1 T S \<Omega> V m n)) (inputs M2)) - (TS M2 M1 T S \<Omega> V m n)" |
-  "TS M2 M1 T S \<Omega> V m (Suc n) = (TS M2 M1 T S \<Omega> V m n) \<union> (C M2 M1 T S \<Omega> V m (Suc n))" 
+  "RM M2 M1 T \<Omega> V m 0 = {}" |
+  "TS M2 M1 T \<Omega> V m 0 = {}" |
+  "TS M2 M1 T \<Omega> V m (Suc 0) = V" |
+  "C M2 M1 T \<Omega> V m 0 = {}" |
+  "C M2 M1 T \<Omega> V m (Suc 0) = V" |
+  "RM M2 M1 T \<Omega> V m (Suc n) = 
+    {xs' \<in> C M2 M1 T \<Omega> V m (Suc n) .
+      (\<not> (language_state_in M1 (initial M1) {xs'} \<subseteq> language_state_in M2 (initial M2) {xs'}))
+      \<or> (\<forall> io \<in> language_state_in M1 (initial M1) {xs'} .
+          (\<exists> V'' \<in> N io M1 V .  
+            (\<exists> S1 . 
+              (\<exists> vs xs .
+                io = (vs@xs)
+                \<and> mcp (vs@xs) V'' vs
+                \<and> S1 \<subseteq> nodes M2
+                \<and> (\<forall> s1 \<in> S1 . \<forall> s2 \<in> S1 .
+                  s1 \<noteq> s2 \<longrightarrow> 
+                    (\<forall> io1 \<in> RP M2 s1 vs xs V'' .
+                       \<forall> io2 \<in> RP M2 s2 vs xs V'' .
+                         B M1 io1 \<Omega> \<noteq> B M1 io2 \<Omega> ))
+                \<and> m < LB M2 M1 vs xs T S1 \<Omega> V'' ))))}" |
+  "C M2 M1 T \<Omega> V m (Suc n) = (append_set ((C M2 M1 T \<Omega> V m n) - (RM M2 M1 T \<Omega> V m n)) (inputs M2)) - (TS M2 M1 T \<Omega> V m n)" |
+  "TS M2 M1 T \<Omega> V m (Suc n) = (TS M2 M1 T \<Omega> V m n) \<union> (C M2 M1 T \<Omega> V m (Suc n))" 
     
     
 
@@ -334,11 +335,11 @@ qed
 
 lemma C_step : 
   assumes "n > 0"
-  shows "C M2 M1 T S \<Omega> V m (Suc n) \<subseteq> (append_set (C M2 M1 T S \<Omega> V m n) (inputs M2)) - C M2 M1 T S \<Omega> V m n"
+  shows "C M2 M1 T \<Omega> V m (Suc n) \<subseteq> (append_set (C M2 M1 T \<Omega> V m n) (inputs M2)) - C M2 M1 T \<Omega> V m n"
 proof -
-  let ?TS = "\<lambda> n . TS M2 M1 T S \<Omega> V m n"
-  let ?C = "\<lambda> n . C M2 M1 T S \<Omega> V m n"
-  let ?RM = "\<lambda> n . RM M2 M1 T S \<Omega> V m n"
+  let ?TS = "\<lambda> n . TS M2 M1 T \<Omega> V m n"
+  let ?C = "\<lambda> n . C M2 M1 T \<Omega> V m n"
+  let ?RM = "\<lambda> n . RM M2 M1 T \<Omega> V m n"
 
   obtain k where n_def[simp] : "n = Suc k" using assms
     using not0_implies_Suc by blast 
@@ -350,16 +351,16 @@ qed
 
 
 lemma C_extension : 
-  "C M2 M1 T S \<Omega> V m (Suc n) \<subseteq> append_sets V (lists_of_length (inputs M2) n)"
+  "C M2 M1 T \<Omega> V m (Suc n) \<subseteq> append_sets V (lists_of_length (inputs M2) n)"
 proof (induction n)
   case 0
   then show ?case by auto
 next
   case (Suc k)
 
-  let ?TS = "\<lambda> n . TS M2 M1 T S \<Omega> V m n"
-  let ?C = "\<lambda> n . C M2 M1 T S \<Omega> V m n"
-  let ?RM = "\<lambda> n . RM M2 M1 T S \<Omega> V m n"
+  let ?TS = "\<lambda> n . TS M2 M1 T \<Omega> V m n"
+  let ?C = "\<lambda> n . C M2 M1 T \<Omega> V m n"
+  let ?RM = "\<lambda> n . RM M2 M1 T \<Omega> V m n"
 
   have "0 < Suc k" by simp
   have "?C (Suc (Suc k)) \<subseteq> (append_set (?C (Suc k)) (inputs M2)) - ?C (Suc k)" using C_step[OF \<open>0 < Suc k\<close>] by blast
@@ -374,16 +375,16 @@ next
 qed
 
 lemma TS_union : 
-shows "TS M2 M1 T S \<Omega> V m i = (\<Union> j \<in> (set [0..<Suc i]) . C M2 M1 T S \<Omega> V m j)" 
+shows "TS M2 M1 T \<Omega> V m i = (\<Union> j \<in> (set [0..<Suc i]) . C M2 M1 T \<Omega> V m j)" 
 proof (induction i)
   case 0
   then show ?case by auto
 next
   case (Suc i)
 
-  let ?TS = "\<lambda> n . TS M2 M1 T S \<Omega> V m n"
-  let ?C = "\<lambda> n . C M2 M1 T S \<Omega> V m n"
-  let ?RM = "\<lambda> n . RM M2 M1 T S \<Omega> V m n"
+  let ?TS = "\<lambda> n . TS M2 M1 T \<Omega> V m n"
+  let ?C = "\<lambda> n . C M2 M1 T \<Omega> V m n"
+  let ?RM = "\<lambda> n . RM M2 M1 T \<Omega> V m n"
 
   have "?TS (Suc i) = ?TS i \<union> ?C (Suc i)"
     by (metis (no_types) C.simps(2) TS.simps(1) TS.simps(2) TS.simps(3) not0_implies_Suc sup_bot.right_neutral sup_commute)
@@ -397,23 +398,23 @@ qed
 lemma C_disj_le_gz : 
   assumes "i \<le> j"
   and    "0 < i"
-shows "C M2 M1 T S \<Omega> V m i \<inter> C M2 M1 T S \<Omega> V m (Suc j) = {}"
+shows "C M2 M1 T \<Omega> V m i \<inter> C M2 M1 T \<Omega> V m (Suc j) = {}"
 proof -
-  let ?TS = "\<lambda> n . TS M2 M1 T S \<Omega> V m n"
-  let ?C = "\<lambda> n . C M2 M1 T S \<Omega> V m n"
-  let ?RM = "\<lambda> n . RM M2 M1 T S \<Omega> V m n"
+  let ?TS = "\<lambda> n . TS M2 M1 T \<Omega> V m n"
+  let ?C = "\<lambda> n . C M2 M1 T \<Omega> V m n"
+  let ?RM = "\<lambda> n . RM M2 M1 T \<Omega> V m n"
 
   have "Suc 0 < Suc j" using assms(1-2) by auto
   then obtain k where "Suc j = Suc (Suc k)" using not0_implies_Suc by blast 
   then have "?C (Suc j) = (append_set (?C j - ?RM j) (inputs M2))  - ?TS j" using C.simps(3) by blast
   then have "?C (Suc j) \<inter> ?TS j = {}" by blast
-  moreover have "?C i \<subseteq> ?TS j" using assms(1) TS_union[of M2 M1 T S \<Omega> V m j] by fastforce  
+  moreover have "?C i \<subseteq> ?TS j" using assms(1) TS_union[of M2 M1 T \<Omega> V m j] by fastforce  
   ultimately show ?thesis by blast
 qed
 
 lemma C_disj_lt : 
   assumes "i < j"
-shows "C M2 M1 T S \<Omega> V m i \<inter> C M2 M1 T S \<Omega> V m j = {}"
+shows "C M2 M1 T \<Omega> V m i \<inter> C M2 M1 T \<Omega> V m j = {}"
 proof (cases i)
   case 0
   then show ?thesis by auto
@@ -425,13 +426,13 @@ qed
 
 lemma C_disj :
   assumes "i \<noteq> j"
-shows "C M2 M1 T S \<Omega> V m i \<inter> C M2 M1 T S \<Omega> V m j = {}"
+shows "C M2 M1 T \<Omega> V m i \<inter> C M2 M1 T \<Omega> V m j = {}"
   by (metis C_disj_lt Int_commute antisym_conv3 assms)
   
 
 
 
-lemma RM_subset : "RM M2 M1 T S \<Omega> V m i \<subseteq> C M2 M1 T S \<Omega> V m i" 
+lemma RM_subset : "RM M2 M1 T \<Omega> V m i \<subseteq> C M2 M1 T \<Omega> V m i" 
 proof (cases i)
   case 0
   then show ?thesis by auto
@@ -444,11 +445,11 @@ qed
 lemma RM_disj : 
   assumes "i \<le> j"
   and    "0 < i"
-shows "RM M2 M1 T S \<Omega> V m i \<inter> RM M2 M1 T S \<Omega> V m (Suc j) = {}"
+shows "RM M2 M1 T \<Omega> V m i \<inter> RM M2 M1 T \<Omega> V m (Suc j) = {}"
 proof -
-  let ?TS = "\<lambda> n . TS M2 M1 T S \<Omega> V m n"
-  let ?C = "\<lambda> n . C M2 M1 T S \<Omega> V m n"
-  let ?RM = "\<lambda> n . RM M2 M1 T S \<Omega> V m n"
+  let ?TS = "\<lambda> n . TS M2 M1 T \<Omega> V m n"
+  let ?C = "\<lambda> n . C M2 M1 T \<Omega> V m n"
+  let ?RM = "\<lambda> n . RM M2 M1 T \<Omega> V m n"
 
   have "?RM i \<subseteq> ?C i" "?RM (Suc j) \<subseteq> ?C (Suc j)" using RM_subset by blast+
   moreover have "?C i \<inter> ?C (Suc j) = {}" using C_disj_le_gz[OF assms] by assumption
@@ -459,20 +460,20 @@ qed
 
 lemma T_extension : 
   assumes "n > 0"
-  shows "TS M2 M1 T S \<Omega> V m (Suc n) - TS M2 M1 T S \<Omega> V m n \<subseteq> (append_set (TS M2 M1 T S \<Omega> V m n) (inputs M2)) - TS M2 M1 T S \<Omega> V m n"
+  shows "TS M2 M1 T \<Omega> V m (Suc n) - TS M2 M1 T \<Omega> V m n \<subseteq> (append_set (TS M2 M1 T \<Omega> V m n) (inputs M2)) - TS M2 M1 T \<Omega> V m n"
 proof -
-  let ?TS = "\<lambda> n . TS M2 M1 T S \<Omega> V m n"
-  let ?C = "\<lambda> n . C M2 M1 T S \<Omega> V m n"
-  let ?RM = "\<lambda> n . RM M2 M1 T S \<Omega> V m n"
+  let ?TS = "\<lambda> n . TS M2 M1 T \<Omega> V m n"
+  let ?C = "\<lambda> n . C M2 M1 T \<Omega> V m n"
+  let ?RM = "\<lambda> n . RM M2 M1 T \<Omega> V m n"
 
   obtain k where n_def[simp] : "n = Suc k" using assms
     using not0_implies_Suc by blast 
 
   have "?C (Suc n) = (append_set (?C n - ?RM n) (inputs M2)) - ?TS n" using n_def using C.simps(3) by blast
   then have "?C (Suc n) \<subseteq> append_set (?C n) (inputs M2) - ?TS n" by blast
-  moreover have "?C n \<subseteq> ?TS n" using TS_union[of M2 M1 T S \<Omega> V m n] by fastforce
+  moreover have "?C n \<subseteq> ?TS n" using TS_union[of M2 M1 T \<Omega> V m n] by fastforce
   ultimately have "?C (Suc n) \<subseteq> append_set (?TS n) (inputs M2) - ?TS n" by blast
-  moreover have "?TS (Suc n) - ?TS n \<subseteq> ?C (Suc n) " using TS.simps(3)[of M2 M1 T S \<Omega> V m k] using n_def by blast
+  moreover have "?TS (Suc n) - ?TS n \<subseteq> ?C (Suc n) " using TS.simps(3)[of M2 M1 T \<Omega> V m k] using n_def by blast
   ultimately show ?thesis by blast
 qed
 
@@ -483,16 +484,16 @@ lemma append_set_prefix :
   using assms by auto 
 
 
-lemma C_subset : "C M2 M1 T S \<Omega> V m i \<subseteq> TS M2 M1 T S \<Omega> V m i"
+lemma C_subset : "C M2 M1 T \<Omega> V m i \<subseteq> TS M2 M1 T \<Omega> V m i"
   by (simp add: TS_union) 
   
 
 lemma TS_subset :
   assumes "i \<le> j"
-  shows "TS M2 M1 T S \<Omega> V m i \<subseteq> TS M2 M1 T S \<Omega> V m j"
+  shows "TS M2 M1 T \<Omega> V m i \<subseteq> TS M2 M1 T \<Omega> V m j"
 proof -
-  have "TS M2 M1 T S \<Omega> V m i = (\<Union> k \<in> (set [0..<Suc i]) . C M2 M1 T S \<Omega> V m k)" 
-       "TS M2 M1 T S \<Omega> V m j = (\<Union> k \<in> (set [0..<Suc j]) . C M2 M1 T S \<Omega> V m k)" using TS_union by assumption+
+  have "TS M2 M1 T \<Omega> V m i = (\<Union> k \<in> (set [0..<Suc i]) . C M2 M1 T \<Omega> V m k)" 
+       "TS M2 M1 T \<Omega> V m j = (\<Union> k \<in> (set [0..<Suc j]) . C M2 M1 T \<Omega> V m k)" using TS_union by assumption+
   moreover have "set [0..<Suc i] \<subseteq> set [0..<Suc j]" using assms by auto
   ultimately show ?thesis by blast
 qed
@@ -502,23 +503,23 @@ qed
 
 
 lemma C_immediate_prefix_containment :
-  assumes "vs@xs \<in> C M2 M1 T S \<Omega> V m (Suc (Suc i))"
+  assumes "vs@xs \<in> C M2 M1 T \<Omega> V m (Suc (Suc i))"
   and     "xs \<noteq> []"
-shows "vs@(butlast xs) \<in> C M2 M1 T S \<Omega> V m (Suc i) - RM M2 M1 T S \<Omega> V m (Suc i)"
+shows "vs@(butlast xs) \<in> C M2 M1 T \<Omega> V m (Suc i) - RM M2 M1 T \<Omega> V m (Suc i)"
 proof (rule ccontr)
-  let ?TS = "\<lambda> n . TS M2 M1 T S \<Omega> V m n"
-  let ?C = "\<lambda> n . C M2 M1 T S \<Omega> V m n"
-  let ?RM = "\<lambda> n . RM M2 M1 T S \<Omega> V m n"
+  let ?TS = "\<lambda> n . TS M2 M1 T \<Omega> V m n"
+  let ?C = "\<lambda> n . C M2 M1 T \<Omega> V m n"
+  let ?RM = "\<lambda> n . RM M2 M1 T \<Omega> V m n"
 
-  assume "vs @ butlast xs \<notin> C M2 M1 T S \<Omega> V m (Suc i) - RM M2 M1 T S \<Omega> V m (Suc i)"
+  assume "vs @ butlast xs \<notin> C M2 M1 T \<Omega> V m (Suc i) - RM M2 M1 T \<Omega> V m (Suc i)"
 
   have "?C (Suc (Suc i)) \<subseteq> append_set (?C (Suc i) - ?RM (Suc i)) (inputs M2)"
     using C.simps(3) by blast 
   then have "?C (Suc (Suc i)) \<subseteq> append_set (?C (Suc i) - ?RM (Suc i)) UNIV" by blast
   moreover have "vs @ xs \<notin> append_set (?C (Suc i) - ?RM (Suc i)) UNIV"
   proof -
-    have "\<forall>as a. vs @ xs \<noteq> as @ [a] \<or> as \<notin> C M2 M1 T S \<Omega> V m (Suc i) - RM M2 M1 T S \<Omega> V m (Suc i) \<or> a \<notin> UNIV"
-      by (metis \<open>vs @ butlast xs \<notin> C M2 M1 T S \<Omega> V m (Suc i) - RM M2 M1 T S \<Omega> V m (Suc i)\<close> assms(2) butlast_append butlast_snoc)
+    have "\<forall>as a. vs @ xs \<noteq> as @ [a] \<or> as \<notin> C M2 M1 T \<Omega> V m (Suc i) - RM M2 M1 T \<Omega> V m (Suc i) \<or> a \<notin> UNIV"
+      by (metis \<open>vs @ butlast xs \<notin> C M2 M1 T \<Omega> V m (Suc i) - RM M2 M1 T \<Omega> V m (Suc i)\<close> assms(2) butlast_append butlast_snoc)
     then show ?thesis
       by blast
   qed
@@ -532,24 +533,24 @@ qed
   
 (* Lemma 5.5.5 *)
 lemma TS_immediate_prefix_containment :
-  assumes "vs@xs \<in> TS M2 M1 T S \<Omega> V m i"
+  assumes "vs@xs \<in> TS M2 M1 T \<Omega> V m i"
   and     "mcp (vs@xs) V vs"
   and     "0 < i"
-shows "vs@(butlast xs) \<in> TS M2 M1 T S \<Omega> V m i"
+shows "vs@(butlast xs) \<in> TS M2 M1 T \<Omega> V m i"
 proof -
-  let ?TS = "\<lambda> n . TS M2 M1 T S \<Omega> V m n"
-  let ?C = "\<lambda> n . C M2 M1 T S \<Omega> V m n"
-  let ?RM = "\<lambda> n . RM M2 M1 T S \<Omega> V m n"
+  let ?TS = "\<lambda> n . TS M2 M1 T \<Omega> V m n"
+  let ?C = "\<lambda> n . C M2 M1 T \<Omega> V m n"
+  let ?RM = "\<lambda> n . RM M2 M1 T \<Omega> V m n"
 
   obtain j where j_def : "j \<le> i \<and> vs@xs \<in> ?C j" using assms(1)  TS_union[where i=i]
   proof -
-    assume a1: "\<And>j. j \<le> i \<and> vs @ xs \<in> C M2 M1 T S \<Omega> V m j \<Longrightarrow> thesis"
+    assume a1: "\<And>j. j \<le> i \<and> vs @ xs \<in> C M2 M1 T \<Omega> V m j \<Longrightarrow> thesis"
     obtain nn :: "nat set \<Rightarrow> (nat \<Rightarrow> 'a list set) \<Rightarrow> 'a list \<Rightarrow> nat" where
       f2: "\<forall>x0 x1 x2. (\<exists>v3. v3 \<in> x0 \<and> x2 \<in> x1 v3) = (nn x0 x1 x2 \<in> x0 \<and> x2 \<in> x1 (nn x0 x1 x2))"
       by moura
-    have "vs @ xs \<in> UNION (set [0..<Suc i]) (C M2 M1 T S \<Omega> V m)"
-      by (metis \<open>\<And>\<Omega> V T S M2 M1. TS M2 M1 T S \<Omega> V m i = (\<Union>j\<in>set [0..<Suc i]. C M2 M1 T S \<Omega> V m j)\<close> \<open>vs @ xs \<in> TS M2 M1 T S \<Omega> V m i\<close>)
-    then have "nn (set [0..<Suc i]) (C M2 M1 T S \<Omega> V m) (vs @ xs) \<in> set [0..<Suc i] \<and> vs @ xs \<in> C M2 M1 T S \<Omega> V m (nn (set [0..<Suc i]) (C M2 M1 T S \<Omega> V m) (vs @ xs))"
+    have "vs @ xs \<in> UNION (set [0..<Suc i]) (C M2 M1 T \<Omega> V m)"
+      by (metis \<open>\<And>\<Omega> V T S M2 M1. TS M2 M1 T \<Omega> V m i = (\<Union>j\<in>set [0..<Suc i]. C M2 M1 T \<Omega> V m j)\<close> \<open>vs @ xs \<in> TS M2 M1 T \<Omega> V m i\<close>)
+    then have "nn (set [0..<Suc i]) (C M2 M1 T \<Omega> V m) (vs @ xs) \<in> set [0..<Suc i] \<and> vs @ xs \<in> C M2 M1 T \<Omega> V m (nn (set [0..<Suc i]) (C M2 M1 T \<Omega> V m) (vs @ xs))"
       using f2 by blast
     then show ?thesis
       using a1 by (metis (no_types) atLeastLessThan_iff leD not_less_eq_eq set_upt)
@@ -601,11 +602,11 @@ proof -
         by (simp add: butlast_append)
 
       have "Suc n < Suc j" using j_assms by auto
-      have "?C (Suc n) \<subseteq> ?TS j" using TS_union[of M2 M1 T S \<Omega> V m j] \<open>Suc n < Suc j\<close>
+      have "?C (Suc n) \<subseteq> ?TS j" using TS_union[of M2 M1 T \<Omega> V m j] \<open>Suc n < Suc j\<close>
         by (metis UN_upper atLeast_upt lessThan_iff)
       
 
-      have "vs @ butlast xs \<in> TS M2 M1 T S \<Omega> V m j" using \<open>vs@(butlast xs) \<in> ?C (Suc n)\<close> \<open>?C (Suc n) \<subseteq> ?TS j\<close> j_def by auto
+      have "vs @ butlast xs \<in> TS M2 M1 T \<Omega> V m j" using \<open>vs@(butlast xs) \<in> ?C (Suc n)\<close> \<open>?C (Suc n) \<subseteq> ?TS j\<close> j_def by auto
       then show ?thesis using j_def TS_subset[of j i] by blast 
     qed
   qed
@@ -614,10 +615,10 @@ qed
 
 (* corollary 5.5.6 *)
 lemma TS_prefix_containment :
-  assumes "vs@xs \<in> TS M2 M1 T S \<Omega> V m i"
+  assumes "vs@xs \<in> TS M2 M1 T \<Omega> V m i"
   and     "mcp (vs@xs) V vs"
   and     "prefix xs' xs"
-shows "vs@xs' \<in> TS M2 M1 T S \<Omega> V m i"
+shows "vs@xs' \<in> TS M2 M1 T \<Omega> V m i"
 (* Perform induction on length difference, as from each prefix we can deduce the 
    desired property for the prefix one element smaller than it via 5.5.5 *)
 using assms proof (induction "length xs - length xs'" arbitrary: xs')
@@ -647,7 +648,7 @@ next
       then have "k = length xs - length (xs' @ [hd xs''])" using \<open>xs = xs'@xs''\<close> Suc.hyps(2) by auto
       moreover have "prefix (xs' @ [hd xs'']) xs" using \<open>xs = xs'@xs''\<close> \<open>xs'' \<noteq> []\<close>
         by (metis Cons_prefix_Cons list.exhaust_sel prefix_code(1) same_prefix_prefix) 
-      ultimately have "vs @ (xs' @ [hd xs'']) \<in> TS M2 M1 T S \<Omega> V m i" using Suc.hyps(1)[OF _ Suc.prems(1,2)] by simp
+      ultimately have "vs @ (xs' @ [hd xs'']) \<in> TS M2 M1 T \<Omega> V m i" using Suc.hyps(1)[OF _ Suc.prems(1,2)] by simp
       
       
       have "mcp (vs @ xs' @ [hd xs'']) V vs" using \<open>xs = xs'@xs''\<close> \<open>xs'' \<noteq> []\<close> assms(2)
@@ -673,7 +674,7 @@ next
       qed 
       
       
-      then have "vs @ butlast (xs' @ [hd xs'']) \<in> TS M2 M1 T S \<Omega> V m i" using TS_immediate_prefix_containment[OF \<open>vs @ (xs' @ [hd xs'']) \<in> TS M2 M1 T S \<Omega> V m i\<close> _ \<open>0 < i\<close>] by simp
+      then have "vs @ butlast (xs' @ [hd xs'']) \<in> TS M2 M1 T \<Omega> V m i" using TS_immediate_prefix_containment[OF \<open>vs @ (xs' @ [hd xs'']) \<in> TS M2 M1 T \<Omega> V m i\<close> _ \<open>0 < i\<close>] by simp
 
       moreover have "xs' = butlast (xs' @ [hd xs''])" using \<open>xs'' \<noteq> []\<close> by simp
 
@@ -702,33 +703,33 @@ qed
 
 
 lemma C_index :
-  assumes "vs @ xs \<in> C M2 M1 T S \<Omega> V m i"
+  assumes "vs @ xs \<in> C M2 M1 T \<Omega> V m i"
   and     "mcp (vs@xs) V vs"
 shows "Suc (length xs) = i"
 using assms proof (induction xs arbitrary: i rule: rev_induct)
   case Nil 
-  then have "vs @ [] \<in> C M2 M1 T S \<Omega> V m 1" by auto
-  then have "vs @ [] \<in> C M2 M1 T S \<Omega> V m (Suc (length []))" by simp
+  then have "vs @ [] \<in> C M2 M1 T \<Omega> V m 1" by auto
+  then have "vs @ [] \<in> C M2 M1 T \<Omega> V m (Suc (length []))" by simp
   
   show ?case
   proof (rule ccontr)
     assume "Suc (length []) \<noteq> i"
-    moreover have "vs @ [] \<in> C M2 M1 T S \<Omega> V m i \<inter> C M2 M1 T S \<Omega> V m (Suc (length []))" using Nil.prems(1) \<open>vs @ [] \<in> C M2 M1 T S \<Omega> V m (Suc (length []))\<close> by auto
+    moreover have "vs @ [] \<in> C M2 M1 T \<Omega> V m i \<inter> C M2 M1 T \<Omega> V m (Suc (length []))" using Nil.prems(1) \<open>vs @ [] \<in> C M2 M1 T \<Omega> V m (Suc (length []))\<close> by auto
     ultimately show "False" using C_disj by blast
   qed
 next
   case (snoc x xs')
 
-  let ?TS = "\<lambda> n . TS M2 M1 T S \<Omega> V m n"
-  let ?C = "\<lambda> n . C M2 M1 T S \<Omega> V m n"
-  let ?RM = "\<lambda> n . RM M2 M1 T S \<Omega> V m n"
+  let ?TS = "\<lambda> n . TS M2 M1 T \<Omega> V m n"
+  let ?C = "\<lambda> n . C M2 M1 T \<Omega> V m n"
+  let ?RM = "\<lambda> n . RM M2 M1 T \<Omega> V m n"
 
   have "vs @ xs' @ [x] \<notin> V" using snoc.prems(2) by auto  
   then have "vs @ xs' @ [x] \<notin> ?C 1" by auto
   moreover have "vs @ xs' @ [x] \<notin> ?C 0" by auto
   ultimately have "1 < i" using snoc.prems(1) by (metis less_one linorder_neqE_nat) 
 
-  then have "vs @ butlast (xs' @ [x]) \<in> C M2 M1 T S \<Omega> V m (i-1)" 
+  then have "vs @ butlast (xs' @ [x]) \<in> C M2 M1 T \<Omega> V m (i-1)" 
   proof -
     have "Suc 0 < i"
       using \<open>1 < i\<close> by auto
@@ -748,15 +749,15 @@ next
 qed
 
 lemma T_index :
-  assumes "vs @ xs \<in> TS M2 M1 T S \<Omega> V m i"
+  assumes "vs @ xs \<in> TS M2 M1 T \<Omega> V m i"
   and     "mcp (vs@xs) V vs"
 shows "Suc (length xs) \<le> i"
 proof -
-  let ?TS = "\<lambda> n . TS M2 M1 T S \<Omega> V m n"
-  let ?C = "\<lambda> n . C M2 M1 T S \<Omega> V m n"
-  let ?RM = "\<lambda> n . RM M2 M1 T S \<Omega> V m n"
+  let ?TS = "\<lambda> n . TS M2 M1 T \<Omega> V m n"
+  let ?C = "\<lambda> n . C M2 M1 T \<Omega> V m n"
+  let ?RM = "\<lambda> n . RM M2 M1 T \<Omega> V m n"
 
-  obtain j where "j < Suc i" "vs@xs \<in> ?C j" using TS_union[of M2 M1 T S \<Omega> V m i]
+  obtain j where "j < Suc i" "vs@xs \<in> ?C j" using TS_union[of M2 M1 T \<Omega> V m i]
     by (metis (full_types) UN_iff assms(1) atLeastLessThan_iff set_upt) 
   then have "Suc (length xs) = j" using C_index
     using assms(2) by blast
@@ -765,20 +766,20 @@ qed
 
 
 lemma C_extension_options :
-  assumes "vs @ xs \<in> C M2 M1 T S \<Omega> V m i"
+  assumes "vs @ xs \<in> C M2 M1 T \<Omega> V m i"
   and     "mcp (vs @ xs @ [x]) V vs"
   and     "x \<in> inputs M2"
   and     "0 < i"
-shows "vs@xs@[x] \<in> C M2 M1 T S \<Omega> V m (Suc i) \<or> vs@xs \<in> RM M2 M1 T S \<Omega> V m i"
-proof (cases "vs@xs \<in> RM M2 M1 T S \<Omega> V m i")
+shows "vs@xs@[x] \<in> C M2 M1 T \<Omega> V m (Suc i) \<or> vs@xs \<in> RM M2 M1 T \<Omega> V m i"
+proof (cases "vs@xs \<in> RM M2 M1 T \<Omega> V m i")
   case True
   then show ?thesis by auto
 next
   case False
 
-  let ?TS = "\<lambda> n . TS M2 M1 T S \<Omega> V m n"
-  let ?C = "\<lambda> n . C M2 M1 T S \<Omega> V m n"
-  let ?RM = "\<lambda> n . RM M2 M1 T S \<Omega> V m n"
+  let ?TS = "\<lambda> n . TS M2 M1 T \<Omega> V m n"
+  let ?C = "\<lambda> n . C M2 M1 T \<Omega> V m n"
+  let ?RM = "\<lambda> n . RM M2 M1 T \<Omega> V m n"
 
   obtain k where "i = Suc k" using assms(4) using gr0_implies_Suc by blast 
   then have "?C (Suc i) = append_set (?C i - ?RM i) (inputs M2) - ?TS i" using C.simps(3) by blast
@@ -790,7 +791,7 @@ next
   moreover have "vs@xs@[x] \<notin> ?TS i"
   proof (rule ccontr)
     assume "\<not> vs @ xs @ [x] \<notin> ?TS i"
-    then obtain j where "j < Suc i" "vs@xs@[x] \<in> ?C j" using TS_union[of M2 M1 T S \<Omega> V m i] by fastforce
+    then obtain j where "j < Suc i" "vs@xs@[x] \<in> ?C j" using TS_union[of M2 M1 T \<Omega> V m i] by fastforce
     then have "Suc (length (xs@[x])) = j" using C_index assms(2) by blast 
 
     then have "Suc (length (xs@[x])) < Suc i" using \<open>j < Suc i\<close> by auto
@@ -810,21 +811,21 @@ qed
 
 (* Lemma 5.5.7 *)
 lemma TS_non_containment_causes :
-  assumes "vs@xs \<notin> TS M2 M1 T S \<Omega> V m i" 
+  assumes "vs@xs \<notin> TS M2 M1 T \<Omega> V m i" 
   and     "mcp (vs@xs) V vs"
   and     "set xs \<subseteq> inputs M2"
   and     "0 < i"
-shows "(\<exists> xr j . xr \<noteq> xs \<and> prefix xr xs \<and> j \<le> i \<and> vs@xr \<in> RM M2 M1 T S \<Omega> V m j)
-       \<or> (\<exists> xc . xc \<noteq> xs \<and> prefix xc xs \<and> vs@xc \<in> (C M2 M1 T S \<Omega> V m i) - (RM M2 M1 T S \<Omega> V m i))"
+shows "(\<exists> xr j . xr \<noteq> xs \<and> prefix xr xs \<and> j \<le> i \<and> vs@xr \<in> RM M2 M1 T \<Omega> V m j)
+       \<or> (\<exists> xc . xc \<noteq> xs \<and> prefix xc xs \<and> vs@xc \<in> (C M2 M1 T \<Omega> V m i) - (RM M2 M1 T \<Omega> V m i))"
   (is "?PrefPreviouslyRemoved \<or> ?PrefJustContained")
-      "\<not> ((\<exists> xr j . xr \<noteq> xs \<and> prefix xr xs \<and> j \<le> i \<and> vs@xr \<in> RM M2 M1 T S \<Omega> V m j)
-         \<and> (\<exists> xc . xc \<noteq> xs \<and> prefix xc xs \<and> vs@xc \<in> (C M2 M1 T S \<Omega> V m i) - (RM M2 M1 T S \<Omega> V m i)))"
+      "\<not> ((\<exists> xr j . xr \<noteq> xs \<and> prefix xr xs \<and> j \<le> i \<and> vs@xr \<in> RM M2 M1 T \<Omega> V m j)
+         \<and> (\<exists> xc . xc \<noteq> xs \<and> prefix xc xs \<and> vs@xc \<in> (C M2 M1 T \<Omega> V m i) - (RM M2 M1 T \<Omega> V m i)))"
   
 proof -
 
-  let ?TS = "\<lambda> n . TS M2 M1 T S \<Omega> V m n"
-  let ?C = "\<lambda> n . C M2 M1 T S \<Omega> V m n"
-  let ?RM = "\<lambda> n . RM M2 M1 T S \<Omega> V m n"
+  let ?TS = "\<lambda> n . TS M2 M1 T \<Omega> V m n"
+  let ?C = "\<lambda> n . C M2 M1 T \<Omega> V m n"
+  let ?RM = "\<lambda> n . RM M2 M1 T \<Omega> V m n"
 
   show "?PrefPreviouslyRemoved \<or> ?PrefJustContained"
   proof (rule ccontr)
@@ -833,7 +834,7 @@ proof -
 
     have "\<nexists>xr j. prefix xr xs \<and> j \<le> i \<and> vs @ xr \<in> ?RM j" 
     proof 
-      assume "\<exists>xr j. prefix xr xs \<and> j \<le> i \<and> vs @ xr \<in> RM M2 M1 T S \<Omega> V m j"
+      assume "\<exists>xr j. prefix xr xs \<and> j \<le> i \<and> vs @ xr \<in> RM M2 M1 T \<Omega> V m j"
       then obtain xr j where "prefix xr xs" "j \<le> i" "vs @ xr \<in> ?RM j" by blast
       then show "False"
       proof (cases "xr = xs")
@@ -861,7 +862,7 @@ proof -
       proof (induction k)
         case 0
         show ?case using \<open>vs \<in> ?C 1\<close>
-          by (metis "0.prems" DiffI One_nat_def \<open>\<nexists>xr j. prefix xr xs \<and> j \<le> i \<and> vs @ xr \<in> RM M2 M1 T S \<Omega> V m j\<close> append_Nil2 take_0 take_is_prefix)  
+          by (metis "0.prems" DiffI One_nat_def \<open>\<nexists>xr j. prefix xr xs \<and> j \<le> i \<and> vs @ xr \<in> RM M2 M1 T \<Omega> V m j\<close> append_Nil2 take_0 take_is_prefix)  
       next
         case (Suc k)
 
@@ -893,7 +894,7 @@ proof -
           have "vs @ take (Suc k) xs = (vs @ take k xs) @ [xs ! k]"
             by (simp add: \<open>k < length xs\<close> take_Suc_conv_app_nth)
           then show ?thesis
-            using f1 \<open>vs @ take k xs \<in> C M2 M1 T S \<Omega> V m (Suc k) - RM M2 M1 T S \<Omega> V m (Suc k)\<close> by blast
+            using f1 \<open>vs @ take k xs \<in> C M2 M1 T \<Omega> V m (Suc k) - RM M2 M1 T \<Omega> V m (Suc k)\<close> by blast
         qed 
 
         moreover have "vs @ take (Suc k) xs \<notin> ?TS (Suc k)" 
@@ -909,11 +910,11 @@ proof -
 
         ultimately show "vs @ take (Suc k) xs \<in> ?C (Suc (Suc k)) - ?RM (Suc (Suc k))"
           using C.simps(3)
-          by (smt C_extension_options DiffI Suc.prems \<open>\<nexists>xr j. prefix xr xs \<and> j \<le> i \<and> vs @ xr \<in> RM M2 M1 T S \<Omega> V m j\<close> \<open>k < length xs\<close> \<open>last (take (Suc k) xs) \<in> inputs M2\<close> \<open>vs @ take k xs \<in> C M2 M1 T S \<Omega> V m (Suc k)\<close> \<open>vs @ take k xs \<notin> RM M2 M1 T S \<Omega> V m (Suc k)\<close> assms(2) last_snoc mcp_prefix_of_suffix take_Suc_conv_app_nth take_is_prefix zero_less_Suc) 
+          by (smt C_extension_options DiffI Suc.prems \<open>\<nexists>xr j. prefix xr xs \<and> j \<le> i \<and> vs @ xr \<in> RM M2 M1 T \<Omega> V m j\<close> \<open>k < length xs\<close> \<open>last (take (Suc k) xs) \<in> inputs M2\<close> \<open>vs @ take k xs \<in> C M2 M1 T \<Omega> V m (Suc k)\<close> \<open>vs @ take k xs \<notin> RM M2 M1 T \<Omega> V m (Suc k)\<close> assms(2) last_snoc mcp_prefix_of_suffix take_Suc_conv_app_nth take_is_prefix zero_less_Suc) 
       qed
     qed
 
-    then have "vs @ take (i-1) xs \<in> C M2 M1 T S \<Omega> V m i - RM M2 M1 T S \<Omega> V m i" using assms(4)
+    then have "vs @ take (i-1) xs \<in> C M2 M1 T \<Omega> V m i - RM M2 M1 T \<Omega> V m i" using assms(4)
       by (metis One_nat_def Suc_diff_1 Suc_leI le_less) 
     then have "?PrefJustContained"
       by (metis C_subset DiffD1 assms(1) subsetCE take_is_prefix)
@@ -950,7 +951,7 @@ proof -
     have "\<And> n . (n < i) \<Longrightarrow> vs@(take n xs) \<in> ?C (Suc n)"
     proof -    
       fix n assume "n < i"
-      show "vs @ take n xs \<in> C M2 M1 T S \<Omega> V m (Suc n)"
+      show "vs @ take n xs \<in> C M2 M1 T \<Omega> V m (Suc n)"
       proof -
         have "n \<le> length xc"
           using \<open>n < i\<close> \<open>Suc (length xc) = i\<close> less_Suc_eq_le by blast 
@@ -964,12 +965,12 @@ proof -
             by simp
         qed 
         then have "vs @ take n xs \<in> ?TS i"
-          by (meson C_subset DiffD1 TS_prefix_containment \<open>prefix xc xs\<close> \<open>vs @ xc \<in> C M2 M1 T S \<Omega> V m i - RM M2 M1 T S \<Omega> V m i\<close> assms(2) contra_subsetD mcp_prefix_of_suffix same_prefix_prefix)
-        then obtain jn where "jn < Suc i" "vs@(take n xs) \<in> ?C jn" using TS_union[of M2 M1 T S \<Omega> V m i]
+          by (meson C_subset DiffD1 TS_prefix_containment \<open>prefix xc xs\<close> \<open>vs @ xc \<in> C M2 M1 T \<Omega> V m i - RM M2 M1 T \<Omega> V m i\<close> assms(2) contra_subsetD mcp_prefix_of_suffix same_prefix_prefix)
+        then obtain jn where "jn < Suc i" "vs@(take n xs) \<in> ?C jn" using TS_union[of M2 M1 T \<Omega> V m i]
           by (metis UN_iff atLeast_upt lessThan_iff)
         moreover have "mcp (vs @ take n xs) V vs"
           by (meson assms(2) mcp_prefix_of_suffix take_is_prefix) 
-        ultimately have "jn = Suc (length (take n xs))" using C_index[of vs "take n xs" M2 M1 T S \<Omega> V m jn] by auto
+        ultimately have "jn = Suc (length (take n xs))" using C_index[of vs "take n xs" M2 M1 T \<Omega> V m jn] by auto
         then have "jn = Suc n"
           using \<open>length xc \<le> length xs\<close> \<open>n \<le> length xc\<close> by auto 
         then show "vs@(take n xs) \<in> ?C (Suc n)" using \<open>vs@(take n xs) \<in> ?C jn\<close> by auto
@@ -980,7 +981,7 @@ proof -
     have "\<And> n . (n < i) \<Longrightarrow> vs@(take n xs) \<notin> ?RM (Suc n)"
     proof -    
       fix n assume "n < i"
-      show "vs @ take n xs \<notin> RM M2 M1 T S \<Omega> V m (Suc n)"
+      show "vs @ take n xs \<notin> RM M2 M1 T \<Omega> V m (Suc n)"
       proof (cases "n = length xc")
         case True
         then show ?thesis using \<open>vs@xc \<in> ?C i - ?RM i\<close>
@@ -1001,7 +1002,7 @@ proof -
           then have "vs @ (take (Suc n) xs) \<in> ?C (Suc (Suc n))" 
             using \<open>\<And> n . (n < i) \<Longrightarrow> vs@(take n xs) \<in> ?C (Suc n)\<close> by blast
           then have "vs @ butlast (take (Suc n) xs) \<in> ?C (Suc n) - ?RM (Suc n)" 
-            using True C_immediate_prefix_containment[of vs "take (Suc n) xs" M2 M1 T S \<Omega> V m n]
+            using True C_immediate_prefix_containment[of vs "take (Suc n) xs" M2 M1 T \<Omega> V m n]
             by (metis Suc_neq_Zero \<open>prefix xc xs\<close> \<open>xc \<noteq> xs\<close> prefix_Nil take_eq_Nil)
           then show ?thesis
             by (metis DiffD2 Suc_lessD True \<open>length xc \<le> length xs\<close> butlast_snoc less_le_trans take_Suc_conv_app_nth)
@@ -1010,10 +1011,10 @@ proof -
           then have "Suc n = length xc"
             using Suc_lessI \<open>n < length xc\<close> by blast
           then have "vs @ (take (Suc n) xs) \<in> ?C (Suc (Suc n))"
-            using \<open>Suc (length xc) = i\<close> \<open>\<And>n. n < i \<Longrightarrow> vs @ take n xs \<in> C M2 M1 T S \<Omega> V m (Suc n)\<close> 
+            using \<open>Suc (length xc) = i\<close> \<open>\<And>n. n < i \<Longrightarrow> vs @ take n xs \<in> C M2 M1 T \<Omega> V m (Suc n)\<close> 
             by auto 
           then have "vs @ butlast (take (Suc n) xs) \<in> ?C (Suc n) - ?RM (Suc n)" 
-            using False C_immediate_prefix_containment[of vs "take (Suc n) xs" M2 M1 T S \<Omega> V m n]
+            using False C_immediate_prefix_containment[of vs "take (Suc n) xs" M2 M1 T \<Omega> V m n]
             by (metis Suc_neq_Zero \<open>prefix xc xs\<close> \<open>xc \<noteq> xs\<close> prefix_Nil take_eq_Nil)
           then show ?thesis
             by (metis Diff_iff \<open>Suc n = length xc\<close> \<open>length xc \<le> length xs\<close> butlast_take diff_Suc_1)
@@ -1026,7 +1027,7 @@ proof -
     proof -
       have "vs@xr \<in> ?C j" using \<open>vs@xr \<in> ?RM j\<close> RM_subset by blast 
       then show ?thesis using C_index
-        by (metis Suc_le_lessD \<open>\<And>n. n < i \<Longrightarrow> vs @ take n xs \<notin> RM M2 M1 T S \<Omega> V m (Suc n)\<close> \<open>j \<le> i\<close> \<open>prefix xr xs\<close> \<open>vs @ xr \<in> RM M2 M1 T S \<Omega> V m j\<close> append_eq_conv_conj assms(2) mcp_prefix_of_suffix prefix_def) 
+        by (metis Suc_le_lessD \<open>\<And>n. n < i \<Longrightarrow> vs @ take n xs \<notin> RM M2 M1 T \<Omega> V m (Suc n)\<close> \<open>j \<le> i\<close> \<open>prefix xr xs\<close> \<open>vs @ xr \<in> RM M2 M1 T \<Omega> V m j\<close> append_eq_conv_conj assms(2) mcp_prefix_of_suffix prefix_def) 
     qed
  
     have "vs@xr \<notin> ?RM j"
@@ -1041,19 +1042,19 @@ qed
 (* lemma 5.5.8 *)
 lemma TS_non_containment_causes_rev : 
   assumes "mcp (vs@xs) V vs"
-  and "(\<exists> xr j . xr \<noteq> xs \<and> prefix xr xs \<and> j \<le> i \<and> vs@xr \<in> RM M2 M1 T S \<Omega> V m j)
-       \<or> (\<exists> xc . xc \<noteq> xs \<and> prefix xc xs \<and> vs@xc \<in> (C M2 M1 T S \<Omega> V m i) - (RM M2 M1 T S \<Omega> V m i))"
+  and "(\<exists> xr j . xr \<noteq> xs \<and> prefix xr xs \<and> j \<le> i \<and> vs@xr \<in> RM M2 M1 T \<Omega> V m j)
+       \<or> (\<exists> xc . xc \<noteq> xs \<and> prefix xc xs \<and> vs@xc \<in> (C M2 M1 T \<Omega> V m i) - (RM M2 M1 T \<Omega> V m i))"
       (is "?PrefPreviouslyRemoved \<or> ?PrefJustContained")
 
-shows "vs@xs \<notin> TS M2 M1 T S \<Omega> V m i"
+shows "vs@xs \<notin> TS M2 M1 T \<Omega> V m i"
 
   
 proof 
-  let ?TS = "\<lambda> n . TS M2 M1 T S \<Omega> V m n"
-  let ?C = "\<lambda> n . C M2 M1 T S \<Omega> V m n"
-  let ?RM = "\<lambda> n . RM M2 M1 T S \<Omega> V m n"
+  let ?TS = "\<lambda> n . TS M2 M1 T \<Omega> V m n"
+  let ?C = "\<lambda> n . C M2 M1 T \<Omega> V m n"
+  let ?RM = "\<lambda> n . RM M2 M1 T \<Omega> V m n"
 
-  assume "vs @ xs \<in> TS M2 M1 T S \<Omega> V m i" 
+  assume "vs @ xs \<in> TS M2 M1 T \<Omega> V m i" 
 
   have "?PrefPreviouslyRemoved \<Longrightarrow> False"
   proof -
@@ -1066,9 +1067,9 @@ proof
     have "vs@(take (Suc (length xr)) xs) \<notin> ?C (Suc j)" 
     proof -
       have "vs@(take (length xr) xs) \<notin> ?C j - ?RM j"
-        by (metis \<open>prefix xr xs\<close> \<open>vs @ xr \<notin> C M2 M1 T S \<Omega> V m j - RM M2 M1 T S \<Omega> V m j\<close> append_eq_conv_conj prefix_def) 
+        by (metis \<open>prefix xr xs\<close> \<open>vs @ xr \<notin> C M2 M1 T \<Omega> V m j - RM M2 M1 T \<Omega> V m j\<close> append_eq_conv_conj prefix_def) 
       show ?thesis
-        by (smt C_immediate_prefix_containment C_index RM_subset Suc_neq_Zero \<open>prefix xr xs\<close> \<open>vs @ take (length xr) xs \<notin> C M2 M1 T S \<Omega> V m j - RM M2 M1 T S \<Omega> V m j\<close> \<open>vs @ xr \<in> RM M2 M1 T S \<Omega> V m j\<close> assms(1) butlast_take diff_Suc_1 list.size(3) mcp_prefix_of_suffix nat_le_linear subsetCE take_all take_is_prefix)
+        by (smt C_immediate_prefix_containment C_index RM_subset Suc_neq_Zero \<open>prefix xr xs\<close> \<open>vs @ take (length xr) xs \<notin> C M2 M1 T \<Omega> V m j - RM M2 M1 T \<Omega> V m j\<close> \<open>vs @ xr \<in> RM M2 M1 T \<Omega> V m j\<close> assms(1) butlast_take diff_Suc_1 list.size(3) mcp_prefix_of_suffix nat_le_linear subsetCE take_all take_is_prefix)
 
       (* TODO: replace smt call ?
         have "\<forall> x \<in> inputs M2 . vs@(take (length xr) xs)@[x] \<notin> append_set (?C j -?RM j) (inputs M2)"
@@ -1084,7 +1085,7 @@ proof
         then have "x \<in> inputs M2" using assms(2)
           by (metis contra_subsetD in_set_takeD last_in_set snoc_eq_iff_butlast) 
         moreover have "vs@(take (length xr) xs) \<notin> ?C j - ?RM j"
-          by (metis \<open>prefix xr xs\<close> \<open>vs @ xr \<notin> C M2 M1 T S \<Omega> V m j - RM M2 M1 T S \<Omega> V m j\<close> append_eq_conv_conj prefix_def) 
+          by (metis \<open>prefix xr xs\<close> \<open>vs @ xr \<notin> C M2 M1 T \<Omega> V m j - RM M2 M1 T \<Omega> V m j\<close> append_eq_conv_conj prefix_def) 
         ultimately have "vs@(take (length xr) xs)@[x] \<notin> append_set (?C j -?RM j) (inputs M2)" by simp
         moreover have "take (length xr) xs = xr"
           by (metis (no_types) \<open>prefix xr xs\<close> append_eq_conv_conj prefix_def)
@@ -1095,14 +1096,14 @@ proof
     
     have "prefix (take (Suc (length xr)) xs) xs"
       by (simp add: take_is_prefix) 
-    then have "vs@(take (Suc (length xr)) xs) \<in> ?TS i" using TS_prefix_containment[OF \<open>vs @ xs \<in> TS M2 M1 T S \<Omega> V m i\<close> assms(1)] by simp
-    then obtain j' where "j' < Suc i \<and> vs@(take (Suc (length xr)) xs) \<in> ?C j'" using TS_union[of M2 M1 T S \<Omega> V m i] by fastforce
+    then have "vs@(take (Suc (length xr)) xs) \<in> ?TS i" using TS_prefix_containment[OF \<open>vs @ xs \<in> TS M2 M1 T \<Omega> V m i\<close> assms(1)] by simp
+    then obtain j' where "j' < Suc i \<and> vs@(take (Suc (length xr)) xs) \<in> ?C j'" using TS_union[of M2 M1 T \<Omega> V m i] by fastforce
     then have "Suc (Suc (length xr)) = j'" using C_index[of vs "take (Suc (length xr)) xs"]
     proof -
       have "\<not> length xs \<le> length xr"
         by (metis (no_types) \<open>prefix xr xs\<close> \<open>xr \<noteq> xs\<close> append_Nil2 append_eq_conv_conj leD nat_less_le prefix_def prefix_length_le)
       then show ?thesis
-        by (metis (no_types) \<open>\<And>i \<Omega> V T S M2 M1. \<lbrakk>vs @ take (Suc (length xr)) xs \<in> C M2 M1 T S \<Omega> V m i; mcp (vs @ take (Suc (length xr)) xs) V vs\<rbrakk> \<Longrightarrow> Suc (length (take (Suc (length xr)) xs)) = i\<close> \<open>j' < Suc i \<and> vs @ take (Suc (length xr)) xs \<in> C M2 M1 T S \<Omega> V m j'\<close> append_eq_conv_conj assms(1) length_take mcp_prefix_of_suffix min.absorb2 not_less_eq_eq prefix_def)
+        by (metis (no_types) \<open>\<And>i \<Omega> V T S M2 M1. \<lbrakk>vs @ take (Suc (length xr)) xs \<in> C M2 M1 T \<Omega> V m i; mcp (vs @ take (Suc (length xr)) xs) V vs\<rbrakk> \<Longrightarrow> Suc (length (take (Suc (length xr)) xs)) = i\<close> \<open>j' < Suc i \<and> vs @ take (Suc (length xr)) xs \<in> C M2 M1 T \<Omega> V m j'\<close> append_eq_conv_conj assms(1) length_take mcp_prefix_of_suffix min.absorb2 not_less_eq_eq prefix_def)
     qed
     moreover have "Suc (length xr) = j" 
       using \<open>vs@xr \<in> ?RM j\<close> RM_subset C_index
@@ -1134,16 +1135,16 @@ qed
 lemma TS_finite :
   assumes "finite V"
   and     "finite (inputs M2)"
-shows "finite (TS M2 M1 T S \<Omega> V m n)"
+shows "finite (TS M2 M1 T \<Omega> V m n)"
 using assms proof (induction n)
   case 0
   then show ?case by auto
 next
   case (Suc n)
 
-  let ?TS = "\<lambda> n . TS M2 M1 T S \<Omega> V m n"
-  let ?C = "\<lambda> n . C M2 M1 T S \<Omega> V m n"
-  let ?RM = "\<lambda> n . RM M2 M1 T S \<Omega> V m n"
+  let ?TS = "\<lambda> n . TS M2 M1 T \<Omega> V m n"
+  let ?C = "\<lambda> n . C M2 M1 T \<Omega> V m n"
+  let ?RM = "\<lambda> n . RM M2 M1 T \<Omega> V m n"
 
   show ?case
   proof (cases "n=0")
@@ -1164,7 +1165,7 @@ next
       ultimately have "?C (Suc n) \<subseteq> append_set (?TS n) (inputs M2)"
         by blast
       moreover have "finite (append_set (?TS n) (inputs M2))"
-        by (simp add: \<open>finite (TS M2 M1 T S \<Omega> V m n)\<close> assms(2) finite_image_set2) 
+        by (simp add: \<open>finite (TS M2 M1 T \<Omega> V m n)\<close> assms(2) finite_image_set2) 
       ultimately show ?thesis
         using infinite_subset by auto 
     qed
@@ -1176,9 +1177,9 @@ qed
 lemma C_finite :
   assumes "finite V"
   and     "finite (inputs M2)"
-shows "finite (C M2 M1 T S \<Omega> V m n)"
+shows "finite (C M2 M1 T \<Omega> V m n)"
 proof -
-  have "C M2 M1 T S \<Omega> V m n \<subseteq> TS M2 M1 T S \<Omega> V m n"
+  have "C M2 M1 T \<Omega> V m n \<subseteq> TS M2 M1 T \<Omega> V m n"
     by (simp add: C_subset) 
   then show ?thesis using TS_finite[OF assms]
     using Finite_Set.finite_subset by blast 
@@ -1187,91 +1188,112 @@ qed
 
 
 lemma R_union_card_is_suffix_length :
-  assumes "OFSM M"
-  and     "xs \<in> L M"
-shows "sum (\<lambda> q . card (R M q [] xs)) (nodes M) = length xs"
+  assumes "OFSM M2"
+  and     "io@xs \<in> L M2"
+shows "sum (\<lambda> q . card (R M2 q io xs)) (nodes M2) = length xs"
 using assms proof (induction xs rule: rev_induct)
   case Nil
-  have "\<forall> q \<in> nodes M . card (R M q [] []) = 0" by auto
   show ?case
     by (simp add: sum.neutral)
 next
   case (snoc x xs)
 
-  have "finite (nodes M)" using assms by auto
+  have "finite (nodes M2)" using assms by auto
 
-  have R_update : "\<And> q . R M q [] (xs@[x]) = (if (q \<in> io_targets M (initial M) (xs @ [x])) 
-                                    then insert (xs@[x]) (R M q [] xs)   
-                                    else R M q [] xs)" by (auto; presburger)
+  have R_update : "\<And> q . R M2 q io (xs@[x]) = (if (q \<in> io_targets M2 (initial M2) (io @ xs @ [x])) 
+                                    then insert (io@xs@[x]) (R M2 q io xs)   
+                                    else R M2 q io xs)" by (auto; presburger)
 
-  obtain q where "io_targets M (initial M) (xs @ [x]) = {q}"
+  obtain q where "io_targets M2 (initial M2) (io @ xs @ [x]) = {q}"
     by (meson assms(1) io_targets_observable_singleton_ex snoc.prems(2)) 
 
-  then have "R M q [] (xs@[x]) = insert (xs@[x]) (R M q [] xs)" using R_update by auto
-  moreover have "(xs@[x]) \<notin> (R M q [] xs)" by auto
-  ultimately have "card (R M q [] (xs@[x])) = Suc (card (R M q [] xs))"
+  then have "R M2 q io (xs@[x]) = insert (io@xs@[x]) (R M2 q io xs)" using R_update by auto
+  moreover have "(io@xs@[x]) \<notin> (R M2 q io xs)" by auto
+  ultimately have "card (R M2 q io (xs@[x])) = Suc (card (R M2 q io xs))"
     by (metis card_insert_disjoint finite_R) 
 
-  have "q \<in> nodes M"
-    by (metis (full_types) FSM.nodes.initial \<open>io_targets M (initial M) (xs @ [x]) = {q}\<close> insertI1 io_targets_nodes) 
+  have "q \<in> nodes M2"
+    by (metis (full_types) FSM.nodes.initial \<open>io_targets M2 (initial M2) (io@xs @ [x]) = {q}\<close> insertI1 io_targets_nodes) 
 
-  have "\<forall> q' . q' \<noteq> q \<longrightarrow> R M q' [] (xs@[x]) = R M q' [] xs" 
-    using \<open>io_targets M (initial M) (xs @ [x]) = {q}\<close> R_update
+  have "\<forall> q' . q' \<noteq> q \<longrightarrow> R M2 q' io (xs@[x]) = R M2 q' io xs" 
+    using \<open>io_targets M2 (initial M2) (io@xs @ [x]) = {q}\<close> R_update
     by auto  
-  then have "\<forall> q' . q' \<noteq> q \<longrightarrow> card (R M q' [] (xs@[x])) = card (R M q' [] xs)" 
+  then have "\<forall> q' . q' \<noteq> q \<longrightarrow> card (R M2 q' io (xs@[x])) = card (R M2 q' io xs)" 
     by auto
 
-  then have "(\<Sum>q\<in>(nodes M - {q}). card (R M q [] (xs@[x]))) = (\<Sum>q\<in>(nodes M - {q}). card (R M q [] xs))"
+  then have "(\<Sum>q\<in>(nodes M2 - {q}). card (R M2 q io (xs@[x]))) = (\<Sum>q\<in>(nodes M2 - {q}). card (R M2 q io xs))"
     by auto
-  moreover have "(\<Sum>q\<in>nodes M. card (R M q [] (xs@[x]))) = (\<Sum>q\<in>(nodes M - {q}). card (R M q [] (xs@[x]))) + (card (R M q [] (xs@[x])))" 
-                "(\<Sum>q\<in>nodes M. card (R M q [] xs)) = (\<Sum>q\<in>(nodes M - {q}). card (R M q [] xs)) + (card (R M q [] xs))"
+  moreover have "(\<Sum>q\<in>nodes M2. card (R M2 q io (xs@[x]))) = (\<Sum>q\<in>(nodes M2 - {q}). card (R M2 q io (xs@[x]))) + (card (R M2 q io (xs@[x])))" 
+                "(\<Sum>q\<in>nodes M2. card (R M2 q io xs)) = (\<Sum>q\<in>(nodes M2 - {q}). card (R M2 q io xs)) + (card (R M2 q io xs))"
   proof -
     have "\<forall>C c f. (infinite C \<or> (c::'c) \<notin> C) \<or> sum f C = (f c::nat) + sum f (C - {c})"
       by (meson sum.remove)
-    then show "(\<Sum>q\<in>nodes M. card (R M q [] (xs@[x]))) = (\<Sum>q\<in>(nodes M - {q}). card (R M q [] (xs@[x]))) + (card (R M q [] (xs@[x])))"
-              "(\<Sum>q\<in>nodes M. card (R M q [] xs)) = (\<Sum>q\<in>(nodes M - {q}). card (R M q [] xs)) + (card (R M q [] xs))"
-      using \<open>finite (nodes M)\<close> \<open>q \<in> nodes M\<close> by presburger+
+    then show "(\<Sum>q\<in>nodes M2. card (R M2 q io (xs@[x]))) = (\<Sum>q\<in>(nodes M2 - {q}). card (R M2 q io (xs@[x]))) + (card (R M2 q io (xs@[x])))"
+              "(\<Sum>q\<in>nodes M2. card (R M2 q io xs)) = (\<Sum>q\<in>(nodes M2 - {q}). card (R M2 q io xs)) + (card (R M2 q io xs))"
+      using \<open>finite (nodes M2)\<close> \<open>q \<in> nodes M2\<close> by presburger+
   qed 
-  ultimately have "(\<Sum>q\<in>nodes M. card (R M q [] (xs@[x]))) = Suc (\<Sum>q\<in>nodes M. card (R M q [] xs))" 
-    using \<open>card (R M q [] (xs@[x])) = Suc (card (R M q [] xs))\<close> by presburger
+  ultimately have "(\<Sum>q\<in>nodes M2. card (R M2 q io (xs@[x]))) = Suc (\<Sum>q\<in>nodes M2. card (R M2 q io xs))" 
+    using \<open>card (R M2 q io (xs@[x])) = Suc (card (R M2 q io xs))\<close> by presburger
 
-  have "(\<Sum>q\<in>nodes M. card (R M q [] xs)) = length xs" using snoc.IH snoc.prems
-    by (meson language_state_prefix)
+  have "(\<Sum>q\<in>nodes M2. card (R M2 q io xs)) = length xs" 
+    using snoc.IH snoc.prems language_state_prefix[of "io@xs" "[x]" M2 "initial M2"]
+  proof -
+    show ?thesis
+      by (metis (no_types) \<open>(io @ xs) @ [x] \<in> L M2 \<Longrightarrow> io @ xs \<in> L M2\<close> \<open>OFSM M2\<close> \<open>io @ xs @ [x] \<in> L M2\<close> append.assoc snoc.IH)
+  qed 
   
   show ?case
   proof -
     show ?thesis
-      by (metis (no_types) \<open>(\<Sum>q\<in>nodes M. card (R M q [] (xs @ [x]))) = Suc (\<Sum>q\<in>nodes M. card (R M q [] xs))\<close> \<open>(\<Sum>q\<in>nodes M. card (R M q [] xs)) = length xs\<close> length_append_singleton)
+      by (metis (no_types) \<open>(\<Sum>q\<in>nodes M2. card (R M2 q io (xs @ [x]))) = Suc (\<Sum>q\<in>nodes M2. card (R M2 q io xs))\<close> \<open>(\<Sum>q\<in>nodes M2. card (R M2 q io xs)) = length xs\<close> length_append_singleton)
   qed   
-
 qed 
+
+
+
+lemma RP_union_card_is_suffix_length :
+  assumes "OFSM M2"
+  and     "io@xs \<in> L M2"
+  and     "is_det_state_cover M2 V"
+  and     "V'' \<in> Perm V M1"
+shows "\<And> q . card (R M2 q io xs) \<le> card (RP M2 q io xs V'')"
+      "sum (\<lambda> q . card (RP M2 q io xs V'')) (nodes M2) \<ge> length xs" 
+proof -
+  have "sum (\<lambda> q . card (R M2 q io xs)) (nodes M2) = length xs" 
+    using R_union_card_is_suffix_length[OF assms(1,2)] by assumption
+  show "\<And> q . card (R M2 q io xs) \<le> card (RP M2 q io xs V'')"
+    by (metis RP_from_R assms(3) assms(4) card_insert_le eq_iff finite_R) 
+  show "sum (\<lambda> q . card (RP M2 q io xs V'')) (nodes M2) \<ge> length xs"
+    by (metis (no_types, lifting) \<open>(\<Sum>q\<in>nodes M2. card (R M2 q io xs)) = length xs\<close> \<open>\<And>q. card (R M2 q io xs) \<le> card (RP M2 q io xs V'')\<close> sum_mono) 
+qed
+
 
 
 lemma state_repetition_via_long_sequence :
   assumes "OFSM M"
   and     "card (nodes M) \<le> m"
   and     "Suc (m * m) \<le> length xs"
-  and     "xs \<in> L M"
-shows "\<exists> q \<in> nodes M . card (R M q [] xs) > m"
+  and     "vs@xs \<in> L M"
+shows "\<exists> q \<in> nodes M . card (R M q vs xs) > m"
 proof (rule ccontr)
-  assume "\<not> (\<exists>q\<in>nodes M. m < card (R M q [] xs))"
-  then have "\<forall> q \<in> nodes M . card (R M q [] xs) \<le> m" by auto
-  then have "sum (\<lambda> q . card (R M q [] xs)) (nodes M) \<le> sum (\<lambda> q . m) (nodes M)"
+  assume "\<not> (\<exists>q\<in>nodes M. m < card (R M q vs xs))"
+  then have "\<forall> q \<in> nodes M . card (R M q vs xs) \<le> m" by auto
+  then have "sum (\<lambda> q . card (R M q vs xs)) (nodes M) \<le> sum (\<lambda> q . m) (nodes M)"
     by (meson sum_mono) 
   moreover have "sum (\<lambda> q . m) (nodes M) \<le> m * m" 
     using assms(2) by auto 
-  ultimately have "sum (\<lambda> q . card (R M q [] xs)) (nodes M) \<le> m * m" 
+  ultimately have "sum (\<lambda> q . card (R M q vs xs)) (nodes M) \<le> m * m" 
     by presburger
 
-  moreover have "Suc (m*m) \<le> sum (\<lambda> q . card (R M q [] xs)) (nodes M)" 
-    using R_union_card_is_suffix_length[OF assms(1,4)] assms(3) by auto
+  moreover have "Suc (m*m) \<le> sum (\<lambda> q . card (R M q vs xs)) (nodes M)" 
+    using R_union_card_is_suffix_length[OF assms(1), of vs xs] assms(4,3) by auto
   ultimately show "False" by simp
 qed
   
 
 
 
-abbreviation "final_iteration M2 M1 T S \<Omega> V m i \<equiv> TS M2 M1 T S \<Omega> V m i = TS M2 M1 T S \<Omega> V m (Suc i)"
+abbreviation "final_iteration M2 M1 T \<Omega> V m i \<equiv> TS M2 M1 T \<Omega> V m i = TS M2 M1 T \<Omega> V m (Suc i)"
 
 
 (* lemma 5.5.9 *)
@@ -1280,13 +1302,13 @@ lemma final_iteration_ex :
   and     "OFSM M2"
   and     "fault_model M2 M1 m"
   and     "test_tools M2 M1 FAIL PM V V'' \<Omega>"
-  shows "\<exists> i . final_iteration M2 M1 T S \<Omega> V m i"
+  shows "\<exists> i . final_iteration M2 M1 T \<Omega> V m i"
 proof 
   let ?i = "Suc (Suc (m * m))"
 
-  let ?TS = "\<lambda> n . TS M2 M1 T S \<Omega> V m n"
-  let ?C = "\<lambda> n . C M2 M1 T S \<Omega> V m n"
-  let ?RM = "\<lambda> n . RM M2 M1 T S \<Omega> V m n"
+  let ?TS = "\<lambda> n . TS M2 M1 T \<Omega> V m n"
+  let ?C = "\<lambda> n . C M2 M1 T \<Omega> V m n"
+  let ?RM = "\<lambda> n . RM M2 M1 T \<Omega> V m n"
 
 
   (* TODO: extract for reuse if necessary *)
@@ -1301,116 +1323,234 @@ proof
   have "\<forall> seq \<in> ?C ?i . seq \<in> ?RM ?i"
   proof  
     fix seq assume "seq \<in> ?C ?i"
-
-    have "[] \<in> V" using \<open>is_det_state_cover M2 V\<close>
-      using det_state_cover_empty by blast 
-    then obtain vs where "mcp seq V vs" 
-      using mcp_ex[OF _ \<open>finite V\<close>] by blast   
-    then obtain xs where "seq = vs@xs"
-      using prefixE by auto 
-
-    
-    then have "Suc (length xs) = ?i" using C_index
-      using \<open>mcp seq V vs\<close> \<open>seq \<in> C M2 M1 T S \<Omega> V m (Suc (Suc (m * m)))\<close> by blast
-    then have "length xs = Suc (m * m)" by auto
-
     show "seq \<in> ?RM ?i"
     proof -
-      have "?RM ?i =  {xs' \<in> C M2 M1 T S \<Omega> V m ?i .
-                        (\<forall> io \<in> language_state_in M1 (initial M1) {xs'} .
-                          (\<exists> V'' \<in> N io M1 V .  
-                            (\<exists> S1 . 
-                              (\<exists> vs xs .
-                                io = (vs@xs)
-                                \<and> mcp (vs@xs) V'' vs
-                                \<and> S1 \<subseteq> S
-                                \<and> (\<forall> s1 \<in> S1 . \<forall> s2 \<in> S1 .
-                                  s1 \<noteq> s2 \<longrightarrow> 
-                                    (\<forall> io1 \<in> RP M2 s1 vs xs V'' .
-                                       \<forall> io2 \<in> RP M2 s2 vs xs V'' .
-                                         B M1 io1 \<Omega> \<noteq> B M1 io2 \<Omega> ))
-                                \<and> m < LB M2 M1 vs xs T S \<Omega> V'' ))))}" 
-        using RM.simps(2)[of M2 M1 T S \<Omega> V m "Suc (m*m)"] by assumption
 
-      have "(\<forall> io \<in> language_state_in M1 (initial M1) {seq} .
-                          (\<exists> V'' \<in> N io M1 V .  
-                            (\<exists> S1 . 
-                              (\<exists> vs xs .
-                                io = (vs@xs)
-                                \<and> mcp (vs@xs) V'' vs
-                                \<and> S1 \<subseteq> S
-                                \<and> (\<forall> s1 \<in> S1 . \<forall> s2 \<in> S1 .
-                                  s1 \<noteq> s2 \<longrightarrow> 
-                                    (\<forall> io1 \<in> RP M2 s1 vs xs V'' .
-                                       \<forall> io2 \<in> RP M2 s2 vs xs V'' .
-                                         B M1 io1 \<Omega> \<noteq> B M1 io2 \<Omega> ))
-                                \<and> m < LB M2 M1 vs xs T S \<Omega> V'' ))))"
-      proof 
-        fix io assume "io\<in>language_state_in M1 (initial M1) {seq}"
-        then have "io \<in> L M1" 
-          by auto
-        moreover have "is_det_state_cover M2 V" 
-          using assms(4) by auto
-        ultimately obtain V'' where "V'' \<in> N io M1 V" 
-          using N_nonempty[OF _ assms(1-3), of V io] by blast
-
-        let ?S1 = "{}"
-
-        have "V'' \<in> Perm V M1" 
-          using \<open>V'' \<in> N io M1 V\<close> by auto
-
-        have "[] \<in> V''"
-          using \<open>V'' \<in> Perm V M1\<close> assms(4) perm_empty by blast 
-        have "finite V''"
-          using \<open>V'' \<in> Perm V M1\<close> assms(2) assms(4) perm_elem_finite by blast
-        obtain vs where "mcp io V'' vs" 
-          using mcp_ex[OF \<open>[] \<in> V''\<close> \<open>finite V''\<close>] by blast
-
-        obtain xs where "io = (vs@xs)"
-          using \<open>mcp io V'' vs\<close> prefixE by auto  
-
-        have "LB M2 M1 vs xs T ?S1 {} V'' = length io" using R_union_card_is_suffix_length[OF assms(1) \<open>io \<in> L M1\<close>]
-
-        have "m < LB M2 M1 vs xs T ?S1 \<Omega> V''" using R_union_card_is_suffix_length[OF assms(1) \<open>io \<in> L M1\<close>]
-
-
-
-
-
+      have "[] \<in> V" using \<open>is_det_state_cover M2 V\<close>
+        using det_state_cover_empty by blast 
+      then obtain vs where "mcp seq V vs" 
+        using mcp_ex[OF _ \<open>finite V\<close>] by blast   
+      then obtain xs where "seq = vs@xs"
+        using prefixE by auto 
   
+      
+      then have "Suc (length xs) = ?i" using C_index
+        using \<open>mcp seq V vs\<close> \<open>seq \<in> C M2 M1 T \<Omega> V m (Suc (Suc (m * m)))\<close> by blast
+      then have "length xs = Suc (m * m)" by auto
   
-  moreover have "finite (inputs M2)" using assms by auto
-  ultimately have "finite (?C ?i)" using C_finite by blast
- 
-  then show "final_iteration M2 M1 T S \<Omega> V m ?i"
-  proof (cases "C M2 M1 T S \<Omega> V m ?i")
-    case emptyI
-    moreover have "?C (Suc ?i) \<subseteq> append_set (?C ?i) (inputs M2)"
-      using C_step by blast
-    ultimately have "?C (Suc ?i) = {}"
-      by blast 
-    then have "?TS (Suc ?i) = ?TS ?i"
-      using TS.simps(3) by blast 
-    then show ?thesis by blast
-   
-  next
-    case (insertI CS seq)
-    then have "seq \<in> ?C ?i" by blast
-    
-    have "[] \<in> V" using \<open>is_det_state_cover M2 V\<close>
-      using det_state_cover_empty by blast 
-    then obtain vs where "mcp seq V vs" 
-      using mcp_ex[OF _ \<open>finite V\<close>] by blast   
-    then obtain xs where "seq = vs@xs"
-      using prefixE by auto 
+      have RM_def : "?RM ?i =  {xs' \<in> C M2 M1 T \<Omega> V m ?i .
+                          (\<not> (language_state_in M1 (initial M1) {xs'} \<subseteq> language_state_in M2 (initial M2) {xs'}))
+                          \<or> (\<forall> io \<in> language_state_in M1 (initial M1) {xs'} .
+                              (\<exists> V'' \<in> N io M1 V .  
+                                (\<exists> S1 . 
+                                  (\<exists> vs xs .
+                                    io = (vs@xs)
+                                    \<and> mcp (vs@xs) V'' vs
+                                    \<and> S1 \<subseteq> nodes M2
+                                    \<and> (\<forall> s1 \<in> S1 . \<forall> s2 \<in> S1 .
+                                      s1 \<noteq> s2 \<longrightarrow> 
+                                        (\<forall> io1 \<in> RP M2 s1 vs xs V'' .
+                                           \<forall> io2 \<in> RP M2 s2 vs xs V'' .
+                                             B M1 io1 \<Omega> \<noteq> B M1 io2 \<Omega> ))
+            \<and> m < LB M2 M1 vs xs T S1 \<Omega> V'' ))))}"
+      using RM.simps(2)[of M2 M1 T \<Omega> V m "Suc (m*m)"] by assumption
+      
+    have "(\<not> (language_state_in M1 (initial M1) {seq} \<subseteq> language_state_in M2 (initial M2) {seq}))
+          \<or> (\<forall> io \<in> language_state_in M1 (initial M1) {seq} .
+              (\<exists> V'' \<in> N io M1 V .  
+                (\<exists> S1 . 
+                  (\<exists> vs xs .
+                    io = (vs@xs)
+                    \<and> mcp (vs@xs) V'' vs
+                    \<and> S1 \<subseteq> nodes M2
+                    \<and> (\<forall> s1 \<in> S1 . \<forall> s2 \<in> S1 .
+                      s1 \<noteq> s2 \<longrightarrow> 
+                        (\<forall> io1 \<in> RP M2 s1 vs xs V'' .
+                           \<forall> io2 \<in> RP M2 s2 vs xs V'' .
+                             B M1 io1 \<Omega> \<noteq> B M1 io2 \<Omega> ))
+                    \<and> m < LB M2 M1 vs xs T S1 \<Omega> V'' ))))"
+      proof (cases "(\<not> (language_state_in M1 (initial M1) {seq} \<subseteq> language_state_in M2 (initial M2) {seq}))")
+        case True
+        then show ?thesis using RM_def by blast
+      next
+        case False
+        have "(\<forall> io \<in> language_state_in M1 (initial M1) {seq} .
+              (\<exists> V'' \<in> N io M1 V .  
+                (\<exists> S1 . 
+                  (\<exists> vs xs .
+                    io = (vs@xs)
+                    \<and> mcp (vs@xs) V'' vs
+                    \<and> S1 \<subseteq> nodes M2
+                    \<and> (\<forall> s1 \<in> S1 . \<forall> s2 \<in> S1 .
+                      s1 \<noteq> s2 \<longrightarrow> 
+                        (\<forall> io1 \<in> RP M2 s1 vs xs V'' .
+                           \<forall> io2 \<in> RP M2 s2 vs xs V'' .
+                             B M1 io1 \<Omega> \<noteq> B M1 io2 \<Omega> ))
+                    \<and> m < LB M2 M1 vs xs T S1 \<Omega> V'' ))))"
+        proof 
+          fix io assume "io\<in>language_state_in M1 (initial M1) {seq}"
+          then have "io \<in> L M1" 
+            by auto
+          moreover have "is_det_state_cover M2 V" 
+            using assms(4) by auto
+          ultimately obtain V'' where "V'' \<in> N io M1 V" 
+            using N_nonempty[OF _ assms(1-3), of V io] by blast
 
-    
-    then have "Suc (length xs) = ?i" using C_index
-      using \<open>mcp seq V vs\<close> \<open>seq \<in> C M2 M1 T S \<Omega> V m (Suc (Suc (m * m)))\<close> by blast
-    then have "length xs = Suc (m * m)"
+          have "io \<in> L M2" 
+            using \<open>io\<in>language_state_in M1 (initial M1) {seq}\<close> False by auto
 
-    then show ?thesis sorry
+          
+  
+          have "V'' \<in> Perm V M1" 
+            using \<open>V'' \<in> N io M1 V\<close> by auto
+  
+          have "[] \<in> V''"
+            using \<open>V'' \<in> Perm V M1\<close> assms(4) perm_empty by blast 
+          have "finite V''"
+            using \<open>V'' \<in> Perm V M1\<close> assms(2) assms(4) perm_elem_finite by blast
+          obtain vs where "mcp io V'' vs" 
+            using mcp_ex[OF \<open>[] \<in> V''\<close> \<open>finite V''\<close>] by blast
+  
+          obtain xs where "io = (vs@xs)"
+            using \<open>mcp io V'' vs\<close> prefixE by auto  
+  
+          then have "vs@xs \<in> L M1" "vs@xs \<in> L M2"
+            using \<open>io \<in> L M1\<close> \<open>io \<in> L M2\<close> by auto
+
+          have "io \<in> L M1" "map fst io \<in> {seq}"
+            using \<open>io\<in>language_state_in M1 (initial M1) {seq}\<close> by auto
+          then have "map fst io = seq" 
+            by auto
+          then have "map fst io \<in> ?C ?i" 
+            using \<open>seq \<in> ?C ?i\<close> by blast
+          then have "(map fst vs) @ (map fst xs) \<in> ?C ?i" 
+            using \<open>io = (vs@xs)\<close> by (metis map_append) 
+
+          have "mcp' io V'' = vs"
+            using \<open>mcp io V'' vs\<close> mcp'_intro by blast 
+
+          have "mcp' (map fst io) V = (map fst vs)"
+            using \<open>V'' \<in> N io M1 V\<close> \<open>mcp' io V'' = vs\<close> by auto 
+
+          then have "mcp (map fst io) V (map fst vs)"
+            by (metis \<open>\<And>thesis. (\<And>vs. mcp seq V vs \<Longrightarrow> thesis) \<Longrightarrow> thesis\<close> \<open>map fst io = seq\<close> mcp'_intro) 
+          
+          
+          then have "mcp (map fst vs @ map fst xs) V (map fst vs)"
+            by (simp add: \<open>io = vs @ xs\<close>) 
+          
+          then have "Suc (length xs) = ?i" using C_index[OF \<open>(map fst vs) @ (map fst xs) \<in> ?C ?i\<close>] 
+            by simp
+
+          then have "Suc (m * m) \<le> length xs" 
+            by simp
+
+          have "card (nodes M2) \<le> m" using assms(3) by auto
+          obtain q where "q \<in> nodes M2" "m < card (R M2 q vs xs)" 
+            using state_repetition_via_long_sequence[OF assms(2) \<open>card (nodes M2) \<le> m\<close>  \<open>Suc (m * m) \<le> length xs\<close> \<open>vs@xs \<in> L M2\<close>] by blast
+
+          have "m < LB M2 M1 vs xs T {q} \<Omega> V''" 
+          proof -
+            have "card (R M2 q vs xs) \<le> card (RP M2 q vs xs V'')" 
+              using RP_union_card_is_suffix_length(1)[OF assms(2) \<open>vs@xs \<in> L M2\<close> \<open>is_det_state_cover M2 V\<close> \<open>V'' \<in> Perm V M1\<close>] by auto
+            then have "m < card (RP M2 q vs xs V'')" 
+              using \<open>m < card (R M2 q vs xs)\<close> by linarith
+            then have "m < (sum (\<lambda> s . card (RP M2 s vs xs V'')) {q})" 
+              by auto
+            moreover have "(sum (\<lambda> s . card (RP M2 s vs xs V'')) {q}) \<le> LB M2 M1 vs xs T {q} \<Omega> V''"
+              by auto
+            ultimately show ?thesis 
+              by linarith 
+          qed
+
+
+          show "\<exists>V''\<in>N io M1 V.
+                 \<exists>S1 vs xs.
+                    io = vs @ xs \<and>
+                    mcp (vs @ xs) V'' vs \<and>
+                    S1 \<subseteq> nodes M2 \<and>
+                    (\<forall>s1\<in>S1.
+                        \<forall>s2\<in>S1.
+                           s1 \<noteq> s2 \<longrightarrow>
+                           (\<forall>io1\<in>RP M2 s1 vs xs V''. \<forall>io2\<in>RP M2 s2 vs xs V''. B M1 io1 \<Omega> \<noteq> B M1 io2 \<Omega>)) \<and>
+                    m < LB M2 M1 vs xs T S1 \<Omega> V''"
+          proof -
+            
+            have "io = vs@xs"
+              using \<open>io = vs@xs\<close> by assumption
+            moreover have "mcp (vs@xs) V'' vs"
+              using \<open>io = vs @ xs\<close> \<open>mcp io V'' vs\<close> by presburger 
+            moreover have "{q} \<subseteq> nodes M2" 
+              using \<open>q \<in> nodes M2\<close> by auto
+            moreover have "(\<forall> s1 \<in> {q} . \<forall> s2 \<in> {q} .
+                        s1 \<noteq> s2 \<longrightarrow> 
+                          (\<forall> io1 \<in> RP M2 s1 vs xs V'' .
+                             \<forall> io2 \<in> RP M2 s2 vs xs V'' .
+                               B M1 io1 \<Omega> \<noteq> B M1 io2 \<Omega> ))"
+            proof -
+              have "\<forall> s1 \<in> {q} . \<forall> s2 \<in> {q} . s1 = s2" 
+                by blast
+              then show ?thesis
+                by blast 
+            qed
+            
+            
+            ultimately have RM_body : "io = (vs@xs)
+                      \<and> mcp (vs@xs) V'' vs
+                      \<and> {q} \<subseteq> nodes M2
+                      \<and> (\<forall> s1 \<in> {q} . \<forall> s2 \<in> {q} .
+                        s1 \<noteq> s2 \<longrightarrow> 
+                          (\<forall> io1 \<in> RP M2 s1 vs xs V'' .
+                             \<forall> io2 \<in> RP M2 s2 vs xs V'' .
+                               B M1 io1 \<Omega> \<noteq> B M1 io2 \<Omega> ))
+                      \<and> m < LB M2 M1 vs xs T {q} \<Omega> V'' " using \<open>m < LB M2 M1 vs xs T {q} \<Omega> V''\<close> 
+              by linarith 
+
+            show ?thesis using \<open>V''\<in>N io M1 V\<close> RM_body
+              by metis 
+          qed
+        qed
+
+        then show ?thesis by metis
+      qed
+
+      then have "seq \<in> {xs' \<in> C M2 M1 T \<Omega> V m (Suc (Suc (m * m))).
+                         \<not> language_state_in M1 (initial M1) {xs'} \<subseteq> language_state_in M2 (initial M2) {xs'} \<or>
+                         (\<forall>io\<in>language_state_in M1 (initial M1) {xs'}.
+                             \<exists>V''\<in>N io M1 V.
+                                \<exists>S1 vs xs.
+                                   io = vs @ xs \<and>
+                                   mcp (vs @ xs) V'' vs \<and>
+                                   S1 \<subseteq> nodes M2 \<and>
+                                   (\<forall>s1\<in>S1.
+                                       \<forall>s2\<in>S1.
+                                          s1 \<noteq> s2 \<longrightarrow>
+                                          (\<forall>io1\<in>RP M2 s1 vs xs V''. \<forall>io2\<in>RP M2 s2 vs xs V''. B M1 io1 \<Omega> \<noteq> B M1 io2 \<Omega>)) \<and>
+                                   m < LB M2 M1 vs xs T S1 \<Omega> V'')}" 
+        using \<open>seq \<in> ?C ?i\<close> by blast
+
+
+      then show ?thesis using RM_def by blast
+    qed
   qed
+
+  then have "?C ?i - ?RM ?i = {}" 
+    by blast
+
+  have "?C (Suc ?i) = append_set (?C ?i - ?RM ?i) (inputs M2) - ?TS ?i"
+    using C.simps(3) by blast 
+
+      
+        
+
+  then have "?C (Suc ?i) = {}" using \<open>?C ?i - ?RM ?i = {}\<close> 
+    by blast
+  then have "?TS (Suc ?i) = ?TS ?i"
+    using TS.simps(3) by blast 
+  then show "final_iteration M2 M1 T \<Omega> V m ?i"
+    by blast 
+qed
+        
 
 
 end
